formal/inference/Inference.thy
@@ -228,7 +228,7 @@ definition make_distinct :: "iEFSM option \<Rightarrow> iEFSM option" where
 function resolve_nondeterminism :: "nondeterministic_pair list \<Rightarrow> iEFSM \<Rightarrow> iEFSM \<Rightarrow> update_modifier \<Rightarrow> (transition_matrix \<Rightarrow> bool) \<Rightarrow> iEFSM option" where
   "resolve_nondeterminism [] _ new _ check = (if deterministic new \<and> check (tm new) then Some new else None)" |
   "resolve_nondeterminism ((from, (dest\<^sub>1, dest\<^sub>2), ((t\<^sub>1, u\<^sub>1), (t\<^sub>2, u\<^sub>2)))#ss) oldEFSM newEFSM m check = (let
-     destMerge = merge_states (dest u\<^sub>1 newEFSM) (dest u\<^sub>2 newEFSM) newEFSM
+     destMerge = merge_states dest\<^sub>1 dest\<^sub>2 newEFSM
      in
      case make_distinct (merge_transitions oldEFSM destMerge t\<^sub>1 u\<^sub>1 t\<^sub>2 u\<^sub>2 m) of
        None \<Rightarrow> resolve_nondeterminism ss oldEFSM newEFSM m check |
